\documentclass[12pt]{article}



\usepackage{amsmath}

\usepackage{amssymb}

\usepackage{tikz}

\usepackage{circuitikz}



\begin{document}



\begin{figure}[h!]

  \begin{center}

    \begin{circuitikz}

     %Loop 1

      \draw (0,0)

      to[V,v=$V(t)$] (0,4) % The voltage source

      to[L=$L_1$] (4,4) % L1

      to[C=$C_1$] (4,0) % C1

      to[R=$R_1$] (0,0); % R1

     %Loop 2 

      \draw (4,4)

      to[L=$L_2$] (8,4) % L2

      to[C=$C_2$] (8,0) % C2

      to[R=$R_2$] (4,0); % R2

     %Loop 3 

      \draw (8,4)

      to[L=$L_3$] (12,4) % L3

      to[C=$C_3$] (12,0) % C3

      to[R=$R_3$] (8,0); % R3

    \end{circuitikz}

    \caption{RLC Circuit diagram}

  \end{center}

\end{figure}



Loop ABGH

	\begin{equation*}	
	V(t)-L_1 \frac{d}{dt}(i_1 + i_2 + i_3)-\frac{q_1}{C_1}-(i_1 + i_2 + i_3)R_1=0
	\end{equation*}

Loop BCFG

	\begin{equation*}
	\frac{q_1}{C_1}-L_2 \frac{d}{dt}(i_2+i_3)-\frac{q_2}{C_2}-(i_2+i_3)R_2=0
	\end{equation*}

Loop CDEF

	\begin{equation*}
	\frac{q_2}{C_2}-L_3 \frac{d}{dt}i_3 -\frac{q_3}{C_3}-i_3 R_3=0
	\end{equation*}



However: $i_k = \frac{dq_k}{dt} ; k=1,2,3$



\begin{align}
	V(t)-&L_1 \frac{d^2}{dt^2}(q_1 + q_2 + q_3)-\frac{q_1}{C_1} -\frac{d}{dt}(q_1 + q_2 + q_3)R_1=0\\ 
	\frac{q_1}{C_1}-&L_2 \frac{d^2}{dt^2}(q_2+q_3)-\frac{q_2}{C_2} -\frac{d}{dt}(q_2+q_3)R_2=0 \label{2} \\ 
	\frac{q_2}{C_2}-&L_3 \frac{d^2}{dt^2}(q_3)-\frac{q_3}{C_3} -\frac{d}{dt}(q_3)R_3=0 \label{3}	
\end{align}

\begin{center}

	\begin{align*}
	q_k(0)&=0, k=1,2,3\\
	i_k(0)=q'_k(0)&=0, k=1,2,3
	\end{align*}

\end{center}

\newpage

\begin{align*}
	y:\left[0;\tau \right]&\rightarrow \mathbb{R}^n\\
	y'(t)&=f\left(t;y(t)\right) ; t\in \left[0;\tau \right]\\
	y(0)&=y_0\\
	q(t)&=(q_1(t);q_2(t);q_3(t)) ; t\in \left[0;\tau \right];
\end{align*}





Let us compute: $L_2(1)-L_1(2)$

\begin{align*}
	&\left( L_2 V-L_2 L_1 \frac{d^2}{dt^2}(q_1+q_2+q_3)-\frac{L_2 q_1}{C_1}-L_2 R_1\frac{d}{dt}(q_1+q_2+q_3)\right)\\ 
	&-\left( \frac{L_1 q_1}{C_1} -L_2 L_1 \frac{d^2}{dt^2}(q_2+q_3)-\frac{L_1 q_2}{C_2} -L_1 R_2 \frac{d}{dt}(q_2+q_3)\right)=0
\end{align*}



\begin{align*}
	L_1 L_2 \frac{d^2 q_1}{dt^2}&=\left[ L_2 V -\frac{L_2 q_1}{C_1}-L_2 R_1 \frac{d}{dt}(q_1+q_2+q_3)\right]\\
	&-\left[\frac{L_1 q_1}{C_1}-\frac{L_1 q_2}{C_2}-L_1 R_2 \frac{d}{dt}(q_2+q_3)\right]\\
	\\    
	L_1 L_2 \frac{d^2 q_1}{dt^2}&=L_2 V -\left(\frac{L_2+L_1}{C_1}\right)q_1+\frac{L_1}{C_2}q_2\\
	&-L_2 R_1\frac{dq_1}{dt}+(L_1 R_2-L_2 R_1)\left(\frac{dq_2}{dt}+\frac{dq_3}{dt}\right)
\end{align*}

\begin{itemize}

	\item $\dfrac{d^2}{dt^2} q_1 = \dfrac{V}{L_1} \ - \ \left( \dfrac{L_2 + L_1}{C_1 L_1 L_2} \right) q_1 \ + \ \dfrac{1}{L_2 C_2} q_2 \ - \ \dfrac{R_1}{L_1} \dfrac{dq_1}{dt} \ - \ \left( \dfrac{L_2}{R_2} - \dfrac{L_1}{R_1} \right) \left( \dfrac{dq_2}{dt} + \dfrac{dq_3}{dt} \right)$\\

	$L_3*\eqref{2} - L_2*\eqref{3} =$ \\\\ $\left( L_3 \dfrac{q_1}{C_1} \ - \ L_2 L_3 \dfrac{d^2}{dt^2} (q_2 + q_3) \ - \ \dfrac{L_3 \ q_2}{C_2} \ - \ L_3 R_2 \dfrac{d}{dt} (q_2 + q_3) \right)$ \begin{flushright}
	$- \ \left( \dfrac{L_2\  q_2}{C_2} \ - \ L_2 L_3 \dfrac{d^2}{dt^2} q_3 \ - \ \dfrac{L_2 \ q_3}{C_3} \ - \ R_3 L_2 \dfrac{d}{dt} q_3 \right) = 0$
\end{flushright} 
	$L_2 L_3 \dfrac{d^2}{dt^2} q_2 \ = \ \dfrac{L_3}{C_1} q_1 \ - \ \dfrac{L_3 \ q_2}{C_2} \ - \ L_3 R_2 \left( \dfrac{dq_2}{dt} +  \dfrac{dq_3}{dt} \right) - \dfrac{L_2 \ q_2}{C_2} + \dfrac{L_2 \ q_3}{C_3} $ 
\begin{flushright}
	$= \ \dfrac{L_3}{C_1} q_1 \ - \ \left( \dfrac{L_2 + L_3}{C_2} \right) q_2 \ + \ \dfrac{L_2}{C_3} q_3 \ - \ L_3 R_2 \left( \dfrac{dq_2}{dt} + \dfrac{dq_3}{dt} \right)$
\end{flushright}

	\item $\dfrac{d^2}{dt^2} q_2 \ = \ \dfrac{q_1}{L_2 C_1} \ - \ \left( \dfrac{L_2 + L_3}{C_2 L_2 L_3} \right) q_2 \ + \ \dfrac{q_3}{C_3 L_3} \ - \ \dfrac{R_2}{L_2} \left( \dfrac{dq_2}{dt} + \dfrac{dq_3}{dt} \right)$\\
	
De \eqref{3}:

	$\dfrac{q_2}{C_2} \ - \ \dfrac{q_3}{C_3} \ - \ R_3 \dfrac{dq_3}{dt} \ = \ L_3 \dfrac{d^2}{dt^2} q_3$\\

	\item $\dfrac{d^2}{dt^2} q_3 \ = \ \dfrac{q_2}{L_3 C_2} \ - \ \dfrac{q_3}{L_3 C_3} - \dfrac{R_3}{L_3} \dfrac{dq_3}{dt}$\\
\end{itemize}

Por lo tanto:

\begin{align*}
	\dfrac{d^2}{dt^2} q_1 &= \dfrac{V}{L_1} - \left( \dfrac{L_2 + L_1}{C_1 L_1 L_2} \right) q_1 + \dfrac{1}{L_2 C_2} q_2 - \dfrac{R_1}{L_1} \dfrac{dq_1}{dt} - \left( \dfrac{L_2}{R_2} - \dfrac{L_1}{R_1} \right) \left( \dfrac{dq_2}{dt} + \dfrac{dq_3}{dt} \right) \\
	\dfrac{d^2}{dt^2} q_2 &= \ \dfrac{q_1}{L_2 C_1} \ - \ \left( \dfrac{L_2 + L_3}{C_2 L_2 L_3} \right) q_2 \ + \ \dfrac{q_3}{C_3 L_3} \ - \ \dfrac{R_2}{L_2} \left( \dfrac{dq_2}{dt} + \dfrac{dq_3}{dt} \right) \\
	\dfrac{d^2}{dt^2} q_3 &= \ \dfrac{q_2}{L_3 C_2} \ - \ \dfrac{q_3}{L_3 C_3} - \dfrac{R_3}{L_3} \dfrac{dq_3}{dt}
\end{align*}

	$$q''(t) = \left[ \begin{array}{l} 
		\dfrac{d^2}{dt^2} q_1 \\\\ 
		\dfrac{d^2}{dt^2} q_2 \\\\ 
		\dfrac{d^2}{dt^2} q_3
	\end{array}
	\right] = g(t, q'(t), q(t)), \ t \in [0, T]$$
	$$q(t) = 0 \qquad q'(t) = 0$$

\end{document}















